renaming and changed use of In to ∉

.Makefile.coq.d
@@ -1,9 +1,9 @@
-src/lang/subst_map.vo src/lang/subst_map.glob src/lang/subst_map.v.beautified src/lang/subst_map.required_vo: src/lang/subst_map.v 
-src/lang/subst_map.vio: src/lang/subst_map.v 
-src/lang/subst_map.vos src/lang/subst_map.vok src/lang/subst_map.required_vos: src/lang/subst_map.v 
-src/lang/hazel.vo src/lang/hazel.glob src/lang/hazel.v.beautified src/lang/hazel.required_vo: src/lang/hazel.v src/lang/subst_map.vo
-src/lang/hazel.vio: src/lang/hazel.v src/lang/subst_map.vio
-src/lang/hazel.vos src/lang/hazel.vok src/lang/hazel.required_vos: src/lang/hazel.v src/lang/subst_map.vos
-src/logic/interp.vo src/logic/interp.glob src/logic/interp.v.beautified src/logic/interp.required_vo: src/logic/interp.v src/lang/hazel.vo
-src/logic/interp.vio: src/logic/interp.v src/lang/hazel.vio
-src/logic/interp.vos src/logic/interp.vok src/logic/interp.required_vos: src/logic/interp.v src/lang/hazel.vos
+theories/lang/subst_map.vo theories/lang/subst_map.glob theories/lang/subst_map.v.beautified theories/lang/subst_map.required_vo: theories/lang/subst_map.v 
+theories/lang/subst_map.vio: theories/lang/subst_map.v 
+theories/lang/subst_map.vos theories/lang/subst_map.vok theories/lang/subst_map.required_vos: theories/lang/subst_map.v 
+theories/lang/hazel.vo theories/lang/hazel.glob theories/lang/hazel.v.beautified theories/lang/hazel.required_vo: theories/lang/hazel.v theories/lang/subst_map.vo
+theories/lang/hazel.vio: theories/lang/hazel.v theories/lang/subst_map.vio
+theories/lang/hazel.vos theories/lang/hazel.vok theories/lang/hazel.required_vos: theories/lang/hazel.v theories/lang/subst_map.vos
+theories/logic/interp.vo theories/logic/interp.glob theories/logic/interp.v.beautified theories/logic/interp.required_vo: theories/logic/interp.v theories/lang/hazel.vo
+theories/logic/interp.vio: theories/logic/interp.v theories/lang/hazel.vio
+theories/logic/interp.vos theories/logic/interp.vok theories/logic/interp.required_vos: theories/logic/interp.v theories/lang/hazel.vos
